sha/verif_sha_final2.v
@@ -65,6 +65,38 @@ Definition invariant_after_if1 hashed (dd: list Z) c md shmd kv:=
          `(K_vector kv);
          `(memory_block shmd 32 md))))).
 
+(*
+Hint Extern 1 (@field_at _ _ _ _ _ _ |-- @field_at _ _ _ _ ?u _) =>
+    (is_evar u; apply derives_refl) : cancel.
+Hint Extern 1 (@data_at _ _ _ _ _ |-- @data_at _ _ _ ?u _) =>
+    (is_evar u; apply derives_refl) : cancel.
+Hint Extern 1 (@data_at _ _ _ _ _ |-- @field_at _ _ _ nil ?u _) =>
+    (is_evar u; apply derives_refl) : cancel.
+Hint Extern 1 (@field_at _ _ _ nil _ _ |-- @data_at _ _ _ ?u _) =>
+    (is_evar u; apply derives_refl) : cancel.
+*)
+
+Lemma data_at_cancel:
+  forall {cs: compspecs} sh t v p,
+    data_at sh t v p |-- data_at sh t v p.
+Proof. intros. apply derives_refl. Qed.
+Lemma field_at_cancel:
+  forall {cs: compspecs} sh t gfs v p,
+    field_at sh t gfs v p |-- field_at sh t gfs v p.
+Proof. intros. apply derives_refl. Qed.
+
+Lemma data_at_field_at_cancel:
+  forall {cs: compspecs} sh t v p,
+    data_at sh t v p |-- field_at sh t nil v p.
+Proof. intros. apply derives_refl. Qed.
+Lemma field_at_data_at_cancel:
+  forall {cs: compspecs} sh t v p,
+    field_at sh t nil v p |-- data_at sh t v p.
+Proof. intros. apply derives_refl. Qed.
+ 
+Hint Resolve data_at_cancel field_at_cancel
+   data_at_field_at_cancel field_at_data_at_cancel : cancel.
+
 Lemma ifbody_final_if1:
   forall (Espec : OracleKind) (hashed : list int) (md c : val) (shmd : share)
   (dd : list Z) (kv: val)
@@ -175,21 +207,17 @@ forward_call (* sha256_block_data_order (c,p); *)
     field_address t_struct_SHA256state_st [StructField _data] c,
     Tsh, kv).
 {
+  simpl.
   repeat rewrite sepcon_assoc; apply sepcon_derives; [ | cancel].
   unfold data_block.
-  simpl. apply andp_right.
-  apply prop_right.
-  apply isbyte_intlist_to_Zlist.
-  apply derives_refl'.
-  rewrite Zlength_intlist_to_Zlist.
-  rewrite H1'.
-  rewrite <- HU.
-  unfold tarray.
+  rewrite prop_true_andp by apply isbyte_intlist_to_Zlist.
+  autorewrite with sublist.
+  rewrite H1', <- HU. change (LBLOCKz*4)%Z with 64.
   rewrite map_map with (g := Int.repr).
   replace (fun x => Int.repr (Int.unsigned x)) with (@id int) by 
     (extensionality xx; rewrite Int.repr_unsigned; auto).
   rewrite map_id.
-  reflexivity.
+  apply derives_refl.
 }
  simpl map.  (* SHOULD NOT BE NECESSARY *)
  set (pad := (CBLOCKz - (ddlen+1))%Z) in *.
@@ -316,6 +344,7 @@ rewrite memory_block_size_compatible
   by (compute; auto).
 normalize.
 rewrite memory_block_data_at_; [ cancel | ].
+apply derives_refl.
 repeat split; auto; try reflexivity.
 apply align_compatible_tarray_tuchar.
 *
